adding conditions for source_in and target_in

fr.inria.atlanmod.coqtl.coq/core/Semantics.v
@@ -17,28 +17,28 @@ Context {tc: TransformationConfiguration}.
 
 (** * Instantiate **)
 
-Definition matchRuleOnPattern (r: Rule) (sm : SourceModel) (sp: list SourceNode) : bool :=
+Definition matchRuleOnPattern (r: Rule) (sm : SourceGraph) (sp: list SourceNode) : bool :=
   match evalGuardExpr r sm sp with Some true => true | _ => false end.
 
-Definition matchPattern (tr: Transformation) (sm : SourceModel) (sp: list SourceNode) : list Rule :=
+Definition matchPattern (tr: Transformation) (sm : SourceGraph) (sp: list SourceNode) : list Rule :=
   filter (fun (r:Rule) => matchRuleOnPattern r sm sp) (Transformation_getRules tr).
 
-Definition instantiateNodeOnPattern (o: OutputPatternNode) (sm: SourceModel) (sp: list SourceNode) (iter: nat)
+Definition instantiateNodeOnPattern (o: OutputPatternNode) (sm: SourceGraph) (sp: list SourceNode) (iter: nat)
   : option TargetNode :=
   evalOutputPatternNodeExpr sm sp iter o.
 
-Definition instantiateNodesOnPattern (o: OutputPatternNode) (sm: SourceModel) (sp: list SourceNode):  list TargetNode :=
+Definition instantiateNodesOnPattern (o: OutputPatternNode) (sm: SourceGraph) (sp: list SourceNode):  list TargetNode :=
   flat_map (fun n => optionToList (instantiateNodeOnPattern o sm sp n))
     (seq 0 (evalNodeIteratorExpr o sm sp)).  
 
-Definition instantiateRuleOnPattern (r: Rule) (sm: SourceModel) (sp: list SourceNode) :  list TargetNode :=
+Definition instantiateRuleOnPattern (r: Rule) (sm: SourceGraph) (sp: list SourceNode) :  list TargetNode :=
   flat_map (fun o => instantiateNodesOnPattern o sm sp)
   (Rule_getOutputPatternNodes r).
 
-Definition instantiatePattern (tr: Transformation) (sm : SourceModel) (sp: list SourceNode) : list TargetNode :=
+Definition instantiatePattern (tr: Transformation) (sm : SourceGraph) (sp: list SourceNode) : list TargetNode :=
   flat_map (fun r => instantiateRuleOnPattern r sm sp) (matchPattern tr sm sp).
 
-Definition instantiateRuleOnPatternIterName (r: Rule) (sm: SourceModel) (sp: list SourceNode) (iter: nat) (name: string): option (TargetNode) :=
+Definition instantiateRuleOnPatternIterName (r: Rule) (sm: SourceGraph) (sp: list SourceNode) (iter: nat) (name: string): option (TargetNode) :=
   match (Rule_findOutputPatternNode r name) with
   | Some o =>  instantiateNodeOnPattern o sm sp iter
   | None => None
@@ -46,33 +46,33 @@ Definition instantiateRuleOnPatternIterName (r: Rule) (sm: SourceModel) (sp: lis
 
 (** * Trace **)
 
-Definition traceNodeOnPattern (o: OutputPatternNode) (sm: SourceModel) (sp: list SourceNode) (iter: nat)
+Definition traceNodeOnPattern (o: OutputPatternNode) (sm: SourceGraph) (sp: list SourceNode) (iter: nat)
   : option TraceLink :=
   match (instantiateNodeOnPattern o sm sp iter) with
   | Some e => Some (buildTraceLink (sp, iter, OutputPatternNode_getName o) e)
   | None => None
   end.
 
-Definition traceNodesOnPattern (o: OutputPatternNode) (sm: SourceModel) (sp: list SourceNode):  list TraceLink :=
+Definition traceNodesOnPattern (o: OutputPatternNode) (sm: SourceGraph) (sp: list SourceNode):  list TraceLink :=
   flat_map (fun n => optionToList (traceNodeOnPattern o sm sp n))
     (seq 0 (evalNodeIteratorExpr o sm sp)).  
 
-Definition traceRuleOnPattern (r: Rule) (sm: SourceModel) (sp: list SourceNode) :  list TraceLink :=
+Definition traceRuleOnPattern (r: Rule) (sm: SourceGraph) (sp: list SourceNode) :  list TraceLink :=
   flat_map (fun o => traceNodesOnPattern o sm sp)
   (Rule_getOutputPatternNodes r).
 
-Definition tracePattern (tr: Transformation) (sm : SourceModel) (sp: list SourceNode) : list TraceLink :=
+Definition tracePattern (tr: Transformation) (sm : SourceGraph) (sp: list SourceNode) : list TraceLink :=
   flat_map (fun r => traceRuleOnPattern r sm sp) (matchPattern tr sm sp).
 
 Definition maxArity (tr: Transformation) : nat := Transformation_getArity tr.
 
-Definition allTuples (tr: Transformation) (sm : SourceModel) :list (list SourceNode) :=
+Definition allTuples (tr: Transformation) (sm : SourceGraph) :list (list SourceNode) :=
   tuples_up_to_n (allNodes sm) (maxArity tr).
 
-Definition trace (tr: Transformation) (sm : SourceModel) : list TraceLink :=
+Definition trace (tr: Transformation) (sm : SourceGraph) : list TraceLink :=
   flat_map (tracePattern tr sm) (allTuples tr sm).  
 
-Definition resolveIter (tls: list TraceLink) (sm: SourceModel) (name: string)
+Definition resolveIter (tls: list TraceLink) (sm: SourceGraph) (name: string)
             (sp: list SourceNode)
             (iter : nat) : option TargetNode :=
 let tl := find (fun tl: TraceLink => 
@@ -84,27 +84,27 @@ match tl with
   | None => None
 end.
 
-Definition resolve (tr: list TraceLink) (sm: SourceModel) (name: string)
+Definition resolve (tr: list TraceLink) (sm: SourceGraph) (name: string)
   (sp: list SourceNode) : option TargetNode :=
   resolveIter tr sm name sp 0.
 
-Definition resolveAllIter (tr: list TraceLink) (sm: SourceModel) (name: string)
+Definition resolveAllIter (tr: list TraceLink) (sm: SourceGraph) (name: string)
   (sps: list(list SourceNode)) (iter: nat)
   : option (list TargetNode) :=
   Some (flat_map (fun l:(list SourceNode) => optionToList (resolveIter tr sm name l iter)) sps).
 
-Definition resolveAll (tr: list TraceLink) (sm: SourceModel) (name: string)
+Definition resolveAll (tr: list TraceLink) (sm: SourceGraph) (name: string)
   (sps: list(list SourceNode)) : option (list TargetNode) :=
   resolveAllIter tr sm name sps 0.
 
-Definition maybeResolve (tr: list TraceLink) (sm: SourceModel) (name: string)
+Definition maybeResolve (tr: list TraceLink) (sm: SourceGraph) (name: string)
   (sp: option (list SourceNode)) : option TargetNode :=
   match sp with 
   | Some sp' => resolve tr sm name sp'
   | None => None
   end.
 
-Definition maybeResolveAll (tr: list TraceLink) (sm: SourceModel) (name: string)
+Definition maybeResolveAll (tr: list TraceLink) (sm: SourceGraph) (name: string)
   (sp: option (list (list SourceNode))) : option (list TargetNode) :=
   match sp with 
   | Some sp' => resolveAll tr sm name sp'
@@ -116,14 +116,14 @@ Definition maybeResolveAll (tr: list TraceLink) (sm: SourceModel) (name: string)
 Definition applyEdgeOnPattern
             (oper: OutputPatternEdge)
             (tr: Transformation)
-            (sm: SourceModel)
+            (sm: SourceGraph)
             (sp: list SourceNode) (iter: nat) (te: TargetNode) (iterl: nat): option TargetEdge :=
   evalOutputPatternEdgeExpr iterl sm sp te iter (trace tr sm) oper.
 
 Definition applyEdgesOnPattern
   (oper: OutputPatternEdge)
   (tr: Transformation)
-  (sm: SourceModel)
+  (sm: SourceGraph)
   (sp: list SourceNode) (iter: nat) (te: TargetNode): list TargetEdge :=
   flat_map (fun n => optionToList (applyEdgeOnPattern oper tr sm sp iter te n))
     (seq 0 (evalLinkIteratorExpr oper sm sp te iter (trace tr sm))).  
@@ -131,7 +131,7 @@ Definition applyEdgesOnPattern
 Definition applyNodeOnPattern
             (ope: OutputPatternNode)
             (tr: Transformation)
-            (sm: SourceModel)
+            (sm: SourceGraph)
             (sp: list SourceNode) (iter: nat) : list TargetEdge :=
   flat_map (fun oper => 
     match (evalOutputPatternNodeExpr sm sp iter ope) with 
@@ -139,20 +139,20 @@ Definition applyNodeOnPattern
     | None => nil
     end) (OutputPatternNode_getOutputEdges ope).
 
-Definition applyNodesOnPattern (o: OutputPatternNode) (tr: Transformation) (sm: SourceModel) (sp: list SourceNode):  list TargetEdge :=
+Definition applyNodesOnPattern (o: OutputPatternNode) (tr: Transformation) (sm: SourceGraph) (sp: list SourceNode):  list TargetEdge :=
   flat_map (fun n => applyNodeOnPattern o tr sm sp n)
     (seq 0 (evalNodeIteratorExpr o sm sp)).  
 
-Definition applyRuleOnPattern (r: Rule) (tr: Transformation) (sm: SourceModel) (sp: list SourceNode) :  list TargetEdge :=
+Definition applyRuleOnPattern (r: Rule) (tr: Transformation) (sm: SourceGraph) (sp: list SourceNode) :  list TargetEdge :=
   flat_map (fun o => applyNodesOnPattern o tr sm sp)
   (Rule_getOutputPatternNodes r).
 
-Definition applyPattern (tr: Transformation) (sm : SourceModel) (sp: list SourceNode) : list TargetEdge :=
+Definition applyPattern (tr: Transformation) (sm : SourceGraph) (sp: list SourceNode) : list TargetEdge :=
   flat_map (fun r => applyRuleOnPattern r tr sm sp) (matchPattern tr sm sp).
 
 (** * Execute **)
 
-Definition execute (tr: Transformation) (sm : SourceModel) : TargetModel :=
+Definition execute (tr: Transformation) (sm : SourceGraph) : TargetGraph :=
   Build_Graph
     (* elements *) (flat_map (instantiatePattern tr sm) (allTuples tr sm))
     (* links *) (flat_map (applyPattern tr sm) (allTuples tr sm)).
