fr.inria.atlanmod.coqtl.coq/core/modeling/byrule/ByRuleSemantics.v
@@ -14,19 +14,19 @@ Section ByRuleSemantics.
 
 Context {tc: TransformationConfiguration} {mtc: ModelingTransformationConfiguration tc}. 
 
-Definition allNodesOfType (t: SourceModelClass) (sm: SourceModel) : list SourceNode :=
+Definition allNodesOfType (t: SourceGraphClass) (sm: SourceGraph) : list SourceNode :=
   filter (hasType t) (allNodes sm).
 
-Definition allNodesOfTypes (l: list SourceModelClass) (sm: SourceModel): list (list SourceNode) :=
-  map (fun t:SourceModelClass => allNodesOfType t sm) l.
+Definition allNodesOfTypes (l: list SourceGraphClass) (sm: SourceGraph): list (list SourceNode) :=
+  map (fun t:SourceGraphClass => allNodesOfType t sm) l.
 
-Definition allTuplesOfTypes (l: list SourceModelClass) (sm: SourceModel): list (list SourceNode) := 
+Definition allTuplesOfTypes (l: list SourceGraphClass) (sm: SourceGraph): list (list SourceNode) := 
   fold_right prod_cons [nil] (allNodesOfTypes l sm).
 
-Definition allTuplesByRule (tr: Transformation) (sm : SourceModel) :list (list SourceNode) :=
+Definition allTuplesByRule (tr: Transformation) (sm : SourceGraph) :list (list SourceNode) :=
   (flat_map (fun (r:Rule) => allTuplesOfTypes (Rule_getInTypes r) sm) (Transformation_getRules tr)).
 
-Definition execute (tr: Transformation) (sm : SourceModel) : TargetModel :=
+Definition execute (tr: Transformation) (sm : SourceGraph) : TargetGraph :=
   Build_Model
     (* elements *) (flat_map (instantiatePattern tr sm) (allTuplesByRule tr sm))
     (* links *) (flat_map (applyPattern tr sm) (allTuplesByRule tr sm)).
