fr.inria.atlanmod.coqtl.coq/core/Schema.v
@@ -1,16 +1,22 @@
 (** * Schema **)
 Require Import core.Graph.
 Require Import core.EqDec.
+Require Import List.
 
 Class Schema :=
 {
     Node: Type;
-    elements_eqdec: EqDec Node;
-    elements_eqb := eq_b;
+    nodes_eqdec: EqDec Node;
+    nodes_eqb := eq_b;
 
     Edge: Type;
-    source: Edge -> Node;
-    target: Edge -> list Node;
 
-    InstanceModel := Graph Node Edge;
+    InstanceGraph := Graph Node Edge;
+
+    source: Edge -> Node;
+    source_in: forall (g: Graph Node Edge) (e: Edge), In e (allEdges g) -> In (source e) (allNodes g);
+
+    target: Edge -> list Node;
+    target_in: forall (g: Graph Node Edge) (e: Edge), In e (allEdges g) -> incl (target e) (allNodes g);
+
 }.
